LeanSubst/Laws.lean
@@ -8,562 +8,564 @@ import LeanSubst.Types.List
 namespace LeanSubst
 
 universe u1 u2 u3
-variable {S : Type u1} {T : Type u2} {U : Type u3}
+variable {S : Type u1} {T T1 T2 : Type u2} {U : Type u3}
+variable {V : List (Type u2)}
 
 @[grind <-]
-theorem Ren.lift_eq_from_eq [RenMap T T] {r : Ren T} {σ : Subst T}
+theorem Ren.lift_eq_from_eq [RenMap T [T]] {r : Ren T} {σ : Subst T}
   : r.to = σ -> r.to.lift = σ.lift
 := by intro h; rw [<-h]
 
-namespace Subst
-  section
-    @[simp]
-    theorem rewrite0 [RenMap T T] : +0σ ∘ +1r = succ T := by
-      congr
+-- namespace Subst
+--   section
+--     @[simp]
+--     theorem rewrite0 [RenMap T [T]] : +0σ ∘ +1r = succ T := by
+--       congr
 
-    @[simp, grind =]
-    theorem rewrite1 : re 0 :: +1σ = id T := by
-      simp [Subst.cons, Subst.id]
-      funext; case _ x =>
-      cases x; all_goals simp
+--     @[simp, grind =]
+--     theorem rewrite1 : re 0 :: +1σ = id T := by
+--       simp [Subst.cons, Subst.id]
+--       funext; case _ x =>
+--       cases x; all_goals simp
 
-    @[simp, grind =]
-    theorem rewrite1_ren : 0 :: +1r = Ren.id T := by
-      simp [Ren.cons, Ren.id]
-      funext; case _ x =>
-      cases x <;> simp
+--     @[simp, grind =]
+--     theorem rewrite1_ren : 0 :: +1r = Ren.id T := by
+--       simp [Ren.cons, Ren.id]
+--       funext; case _ x =>
+--       cases x <;> simp
 
-    open SubstMap
+--     open SubstMap
 
-    @[simp, grind =]
-    theorem I_lift [RenMap T T] {k} : +0σ.lift k = id T := by
-      funext; case _ x =>
-      cases x; all_goals (simp [lift, id, act, SubstAction.act])
-      grind
+--     @[simp, grind =]
+--     theorem I_lift [RenMap T [T]] {k} : +0σ.lift k = id T := by
+--       funext; case _ x =>
+--       cases x; all_goals (simp [lift, id, act, SubstAction.act])
+--       sorry --grind
 
-    @[simp, grind =]
-    theorem rewrite2 [SubstMap T T] {σ : Subst T} : +0σ ∘ σ = σ := by
-      funext; case _ x =>
-      simp [compose, id, act, SubstAction.act]
+--     @[simp, grind =]
+--     theorem rewrite2 [SubstMap T [T]] {σ : Subst T} : +0σ ∘ σ = σ := by
+--       funext; case _ x =>
+--       simp [compose, id, act, SubstAction.act]
+--       sorry
 
-    @[simp, grind =]
-    theorem rewrite2_ren [SubstMap T T] {σ : Subst T} : +0r ∘ σ = σ := by
-      funext; case _ x =>
-      simp [compose_ren_left, act, SubstAction.act]
+--     @[simp, grind =]
+--     theorem rewrite2_ren [SubstMap T [T]] {σ : Subst T} : +0r ∘ σ = σ := by
+--       funext; case _ x =>
+--       simp [compose_ren_left, act, SubstAction.act]
 
-    @[simp, grind =]
-    theorem rewrite3_cons [SubstMap T T] {σ τ : Subst T} {a : Action T}
-      : (a :: σ) ∘ τ = a[τ] :: (σ ∘ τ)
-    := by
-      simp [cons, compose]
-      funext; case _ x =>
-      cases x; all_goals simp [act, SubstAction.act]
+--     @[simp, grind =]
+--     theorem rewrite3_cons [SubstMap T [T]] {σ τ : Subst T} {a : Action T}
+--       : (a :: σ) ∘ τ = a[τ] :: (σ ∘ τ)
+--     := by
+--       simp [cons, compose]
+--       funext; case _ x =>
+--       cases x; all_goals simp [act, SubstAction.act]
 
-    @[simp, grind =]
-    theorem rewrite3_cons_ren [RenMap T T] [SubstMap T T] {σ : Subst T} {r : Ren T} {x : Nat}
-      : (re x :: σ) ∘ r = re (r.act x) :: (σ ∘ r)
-    := by
-      simp [cons, compose_ren_right]
-      funext; case _ x =>
-      cases x; all_goals simp [act, SubstAction.act]
+--     @[simp, grind =]
+--     theorem rewrite3_cons_ren [RenMap T [T]] [SubstMap T [T]] {σ : Subst T} {r : Ren T} {x : Nat}
+--       : (re x :: σ) ∘ r = re (r.act x) :: (σ ∘ r)
+--     := by
+--       simp [cons, compose_ren_right]
+--       funext; case _ x =>
+--       cases x; sorry; all_goals simp [act, SubstAction.act]
 
-    @[simp, grind =]
-    theorem rewrite3_append [SubstMap T T] {σ τ : Subst T} {ℓ : List (Action T)}
-      : (ℓ ++ σ) ∘ τ = ℓ[τ] ++ (σ ∘ τ)
-    := by
-      induction ℓ generalizing σ τ <;> simp
-      case _ hd tl ih =>
-      cases hd <;> simp [*]
+  --   @[simp, grind =]
+  --   theorem rewrite3_append [SubstMap T [T]] {σ τ : Subst T} {ℓ : List (Action T)}
+  --     : (ℓ ++ σ) ∘ τ = ℓ[τ] ++ (σ ∘ τ)
+  --   := by
+  --     induction ℓ generalizing σ τ <;> simp
+  --     case _ hd tl ih =>
+  --     cases hd <;> simp [*]
 
-    @[simp, grind =]
-    theorem rewrite3_append_act [SubstMap T T] {σ τ : Subst T} {ℓ : List Nat}
-      : (ℓ ++ σ) ∘ τ = τ.act ℓ ++ (σ ∘ τ)
-    := by induction ℓ generalizing σ τ <;> simp [*]
+  --   @[simp, grind =]
+  --   theorem rewrite3_append_act [SubstMap T [T]] {σ τ : Subst T} {ℓ : List Nat}
+  --     : (ℓ ++ σ) ∘ τ = τ.act ℓ ++ (σ ∘ τ)
+  --   := by induction ℓ generalizing σ τ <;> simp [*]
 
-    @[simp, grind =]
-    theorem rewrite3_append_ren [RenMap T T] [SubstMap T T] {σ : Subst T} {r : Ren T} {ℓ : List Nat}
-      : (ℓ ++ σ) ∘ r = ℓ⟨r⟩ ++ (σ ∘ r)
-    := by
-      induction ℓ generalizing σ r <;> simp
-      case _ hd tl ih =>
-      cases hd <;> simp [*]
+  --   @[simp, grind =]
+  --   theorem rewrite3_append_ren [RenMap T [T]] [SubstMap T [T]] {σ : Subst T} {r : Ren T} {ℓ : List Nat}
+  --     : (ℓ ++ σ) ∘ r = ℓ⟨r⟩ ++ (σ ∘ r)
+  --   := by
+  --     induction ℓ generalizing σ r <;> simp
+  --     case _ hd tl ih =>
+  --     cases hd <;> simp [*]
 
-    @[simp, grind =]
-    theorem rewrite4_cons [SubstMap T T]  {s} {σ : Subst T} : +1σ ∘ (s :: σ) = σ := by
-      simp [Subst.cons]
-      funext; case _ x =>
-      cases x; all_goals (simp [compose, succ, act, SubstAction.act])
+  --   @[simp, grind =]
+  --   theorem rewrite4_cons [SubstMap T [T]]  {s} {σ : Subst T} : +1σ ∘ (s :: σ) = σ := by
+  --     simp [Subst.cons]
+  --     funext; case _ x =>
+  --     cases x; all_goals (simp [compose, succ, act, SubstAction.act])
 
-    @[simp, grind =]
-    theorem rewrite4_cons_ren [SubstMap T T]  {s} {σ : Subst T} : +1r ∘ (s :: σ) = σ := by
-      simp [Subst.cons]
-      funext; case _ x =>
-      cases x; all_goals (simp [compose_ren_left, act, SubstAction.act])
+  --   @[simp, grind =]
+  --   theorem rewrite4_cons_ren [SubstMap T [T]]  {s} {σ : Subst T} : +1r ∘ (s :: σ) = σ := by
+  --     simp [Subst.cons]
+  --     funext; case _ x =>
+  --     cases x; all_goals (simp [compose_ren_left, act, SubstAction.act])
 
-    @[simp, grind =]
-    theorem rewrite5 [SubstMap T T] {σ : Subst T} : σ.act 0 :: (+1σ ∘ σ) = σ := by
-      simp [Subst.cons, Subst.compose]; congr
-      funext; case _ x =>
-      cases x <;> simp [act, SubstAction.act]
+  --   @[simp, grind =]
+  --   theorem rewrite5 [SubstMap T [T]] {σ : Subst T} : σ.act 0 :: (+1σ ∘ σ) = σ := by
+  --     simp [Subst.cons, Subst.compose]; congr
+  --     funext; case _ x =>
+  --     cases x <;> simp [act, SubstAction.act]
 
-    @[simp, grind =]
-    theorem rewrite5_ren [SubstMap T T] {σ : Subst T} : σ.act 0 :: (+1r ∘ σ) = σ := by
-      simp [Subst.cons]; congr
-      funext; case _ x =>
-      cases x <;> simp [act, SubstAction.act]
-  end
+  --   @[simp, grind =]
+  --   theorem rewrite5_ren [SubstMap T [T]] {σ : Subst T} : σ.act 0 :: (+1r ∘ σ) = σ := by
+  --     simp [Subst.cons]; congr
+  --     funext; case _ x =>
+  --     cases x <;> simp [act, SubstAction.act]
+  -- end
 
-  @[simp, grind =]
-  theorem rewrite_lift [RenMap T T] {σ : Subst T}
-    : σ.lift = re 0 :: (σ ∘ +1r)
-  := by
-    simp [cons, lift, compose_ren_right]
-    funext; case _ x =>
-    cases x <;> simp
+  -- @[simp, grind =]
+  -- theorem rewrite_lift [RenMap T [T]] {σ : Subst T}
+  --   : σ.lift = re 0 :: (σ ∘ +1r)
+  -- := by
+  --   simp [cons, lift, compose_ren_right]
+  --   funext; case _ x =>
+  --   cases x <;> simp
 
-  @[simp, grind =]
-  theorem rewrite_lift_zero [RenMap T T] [RenMapId T T] {σ : Subst T}
-    : σ.lift 0 = σ
-  := by simp [lift, act, SubstAction.act]
+  -- @[simp, grind =]
+  -- theorem rewrite_lift_zero [RenMap T [T]] [RenMapId T T] {σ : Subst T}
+  --   : σ.lift 0 = σ
+  -- := by simp [lift, act, SubstAction.act]
 
-  @[grind =]
-  theorem rewrite_lift_succ
-    [RenMap T T] [RenMapId T T] [RenMapCompose T T]
-    {k} {σ : Subst T}
-    : σ.lift (k + 1) = (σ.lift k).lift
-  := by
-    induction k; simp
-    case _ n ih =>
-      replace ih (i : Nat) : (σ.lift (n + 1)).act i = ((σ.lift n).lift 1).act i := by rw [ih]
-      simp [Subst.lift]
-      funext; case _ i =>
-      have lem := ih i
-      cases i <;> simp [act, SubstAction.act]
-      case _ k =>
-      split <;> simp
-      rw [Ren.compose_add_succ_right]
+  -- @[grind =]
+  -- theorem rewrite_lift_succ
+  --   [RenMap T [T]] [RenMapId T T] [RenMapCompose T T]
+  --   {k} {σ : Subst T}
+  --   : σ.lift (k + 1) = (σ.lift k).lift
+  -- := by
+  --   induction k; simp
+  --   case _ n ih =>
+  --     replace ih (i : Nat) : (σ.lift (n + 1)).act i = ((σ.lift n).lift 1).act i := by rw [ih]
+  --     simp [Subst.lift]
+  --     funext; case _ i =>
+  --     have lem := ih i
+  --     cases i <;> simp [act, SubstAction.act]
+  --     case _ k =>
+  --     split <;> simp
+  --     rw [Ren.compose_add_succ_right]
 
-  @[simp, grind =]
-  theorem rewrite6 [RenMap T T] [SubstMap T T] [SubstMapId T T] {σ : Subst T}
-    : σ ∘ +0σ = σ
-  := by
-    simp [compose, id, act, SubstAction.act]; congr; funext; case _ x =>
-    generalize zdef : σ.inner x = z
-    cases z <;> simp [act, SubstAction.act]
-    case _ t =>
-    have lem : t[id T] = t := by simp
-    simp [id] at lem; exact lem
+  -- @[simp, grind =]
+  -- theorem rewrite6 [RenMap T [T]] [SubstMap T [T]] [SubstMapId T T] {σ : Subst T}
+  --   : σ ∘ +0σ = σ
+  -- := by
+  --   simp [compose, id, act, SubstAction.act]; congr; funext; case _ x =>
+  --   generalize zdef : σ.inner x = z
+  --   cases z <;> simp [act, SubstAction.act]
+  --   case _ t =>
+  --   have lem : t[id T] = t := by simp
+  --   simp [id] at lem; exact lem
 
-  @[simp, grind =]
-  theorem rewrite6_ren [RenMap T T] [RenMapId T T] {σ : Subst T}
-    : σ ∘ +0r = σ
-  := by
-    simp [compose_ren_right]; congr
+  -- @[simp, grind =]
+  -- theorem rewrite6_ren [RenMap T [T]] [RenMapId T T] {σ : Subst T}
+  --   : σ ∘ +0r = σ
+  -- := by
+  --   simp [compose_ren_right]; congr
 
-  @[simp, grind =]
-  theorem rewrite7
-    [SubstMap T T] [SubstMapCompose T T]
-    {σ τ μ : Subst T}
-    : (σ ∘ τ) ∘ μ = σ ∘ τ ∘ μ
-  := by
-    simp [Subst.compose, act, SubstAction.act]
-    funext; case _ x =>
-    cases σ.inner x <;> simp [act, SubstAction.act]
-    simp [compose, act, SubstAction.act]
+  -- @[simp, grind =]
+  -- theorem rewrite7
+  --   [SubstMap T [T]] [SubstMapCompose T T]
+  --   {σ τ μ : Subst T}
+  --   : (σ ∘ τ) ∘ μ = σ ∘ τ ∘ μ
+  -- := by
+  --   simp [Subst.compose, act, SubstAction.act]
+  --   funext; case _ x =>
+  --   cases σ.inner x <;> simp [act, SubstAction.act]
+  --   simp [compose, act, SubstAction.act]
 
-  @[simp, grind =]
-  theorem rewrite7_ren
-    [RenMap T T] [RenMapCompose T T]
-    {σ : Subst T} {r1 r2 : Ren T}
-    : (σ ∘ r1) ∘ r2 = σ ∘ r1 ∘ r2
-  := by simp [compose_ren_right]
+  -- @[simp, grind =]
+  -- theorem rewrite7_ren
+  --   [RenMap T [T]] [RenMapCompose T T]
+  --   {σ : Subst T} {r1 r2 : Ren T}
+  --   : (σ ∘ r1) ∘ r2 = σ ∘ r1 ∘ r2
+  -- := by simp [compose_ren_right]
 
-  @[simp, grind =]
-  theorem rewrite4_append_direct [SubstMap T T] [SubstMapCompose T T]
-    {ℓ : List $ Action T} {σ : Subst T}
-    : (add T ℓ.length) ∘ (ℓ ++ σ) = σ
-  := by
-    induction ℓ generalizing σ <;> simp
-    case _ hd tl ih =>
-    rw [compose_add_succ_right]
-    simp [*]
+  -- @[simp, grind =]
+  -- theorem rewrite4_append_direct [SubstMap T [T]] [SubstMapCompose T T]
+  --   {ℓ : List $ Action T} {σ : Subst T}
+  --   : (add T ℓ.length) ∘ (ℓ ++ σ) = σ
+  -- := by
+  --   induction ℓ generalizing σ <;> simp
+  --   case _ hd tl ih =>
+  --   rw [compose_add_succ_right]
+  --   simp [*]
 
-  @[simp, grind <-]
-  theorem rewrite4_append_indirect [SubstMap T T] [SubstMapCompose T T]
-    {k} {ℓ : List $ Action T} {σ : Subst T} (h : k = ℓ.length)
-    : (add T k) ∘ (ℓ ++ σ) = σ
-  := by subst h; simp
+  -- @[simp, grind <-]
+  -- theorem rewrite4_append_indirect [SubstMap T [T]] [SubstMapCompose T T]
+  --   {k} {ℓ : List $ Action T} {σ : Subst T} (h : k = ℓ.length)
+  --   : (add T k) ∘ (ℓ ++ σ) = σ
+  -- := by subst h; simp
 
-  @[grind =]
-  theorem subst_append_assoc {xs ys : List $ Action T} {σ : Subst T}
-    : xs ++ ys ++ σ = xs ++ (ys ++ σ)
-  := by
-    induction xs generalizing ys σ <;> simp [*]
+  -- @[grind =]
+  -- theorem subst_append_assoc {xs ys : List $ Action T} {σ : Subst T}
+  --   : xs ++ ys ++ σ = xs ++ (ys ++ σ)
+  -- := by
+  --   induction xs generalizing ys σ <;> simp [*]
 
-  @[grind =]
-  theorem subst_append_assoc_nat {xs ys : List Nat} {σ : Subst T}
-    : xs ++ ys ++ σ = xs ++ (ys ++ σ)
-  := by
-    induction xs generalizing ys σ <;> simp [*]
+  -- @[grind =]
+  -- theorem subst_append_assoc_nat {xs ys : List Nat} {σ : Subst T}
+  --   : xs ++ ys ++ σ = xs ++ (ys ++ σ)
+  -- := by
+  --   induction xs generalizing ys σ <;> simp [*]
 
-  @[simp]
-  theorem range_act_succ {s e} {σ : Subst T} : act (succ T) (s..e) ++ σ = s.succ..e.succ ++ σ := by
-    induction e generalizing s σ <;> simp
-    case _ e ih =>
-    simp [Ren.range]
-    cases Nat.decLe s e
-    case _ h2 => simp [ite]
-    case _ h2 =>
-      simp [ite]
-      cases Nat.decLe (s + 1) e
-      case _ h3 =>
-        have lem : s = e := by omega
-        subst lem; simp
-      case _ h3 =>
-        simp [*]
-        rw [subst_append_assoc, ih]; simp
-        rw [subst_append_assoc_nat]; simp [Ren.range]
-        split
-        case _ h4 => rw [subst_append_assoc_nat]; simp
-        case _ h4 => omega
+  -- @[simp]
+  -- theorem range_act_succ {s e} {σ : Subst T} : act (succ T) (s..e) ++ σ = s.succ..e.succ ++ σ := by
+  --   induction e generalizing s σ <;> simp
+  --   case _ e ih =>
+  --   simp [Ren.range]
+  --   cases Nat.decLe s e
+  --   case _ h2 => simp [ite]
+  --   case _ h2 =>
+  --     simp [ite]
+  --     cases Nat.decLe (s + 1) e
+  --     case _ h3 =>
+  --       have lem : s = e := by omega
+  --       subst lem; simp
+  --     case _ h3 =>
+  --       simp [*]
+  --       rw [subst_append_assoc, ih]; simp
+  --       rw [subst_append_assoc_nat]; simp [Ren.range]
+  --       split
+  --       case _ h4 => rw [subst_append_assoc_nat]; simp
+  --       case _ h4 => omega
 
-  @[simp]
-  theorem range_act_succ_ren {s e : Nat} {σ : Subst T}
-    : (s..e)⟨.succ T⟩ ++ σ = s.succ..e.succ ++ σ
-  := by
-    induction e generalizing s σ <;> simp
-    case _ e ih =>
-    simp [Ren.range]
-    cases Nat.decLe s e
-    case _ h2 => simp [ite]
-    case _ h2 =>
-      simp [ite]
-      cases Nat.decLe (s + 1) e
-      case _ h3 =>
-        have lem : s = e := by omega
-        subst lem; simp
-      case _ h3 =>
-        simp [*]
-        rw [subst_append_assoc_nat, ih]; simp
-        rw [subst_append_assoc_nat]; simp [Ren.range]
-        split
-        case _ h4 => rw [subst_append_assoc_nat]; simp
-        case _ h4 => omega
+  -- @[simp]
+  -- theorem range_act_succ_ren {s e : Nat} {σ : Subst T}
+  --   : (s..e)⟨.succ T⟩ ++ σ = s.succ..e.succ ++ σ
+  -- := by
+  --   induction e generalizing s σ <;> simp
+  --   case _ e ih =>
+  --   simp [Ren.range]
+  --   cases Nat.decLe s e
+  --   case _ h2 => simp [ite]
+  --   case _ h2 =>
+  --     simp [ite]
+  --     cases Nat.decLe (s + 1) e
+  --     case _ h3 =>
+  --       have lem : s = e := by omega
+  --       subst lem; simp
+  --     case _ h3 =>
+  --       simp [*]
+  --       rw [subst_append_assoc_nat, ih]; simp
+  --       rw [subst_append_assoc_nat]; simp [Ren.range]
+  --       split
+  --       case _ h4 => rw [subst_append_assoc_nat]; simp
+  --       case _ h4 => omega
 
-  @[simp, grind =]
-  theorem rewrite_lift_k
-    [RenMap T T] [RenMapId T T] [RenMapCompose T T]
-    [SubstMap T T] [SubstMapId T T] [SubstMapCompose T T]
-    {k} {σ : Subst T}
-    : σ.lift k = 0..k ++ (σ ∘ +r k)
-  := by
-    induction k generalizing σ <;> simp
-    case _ k ih =>
-      rw [rewrite_lift_succ, ih]
-      simp; congr
+  -- @[simp, grind =]
+  -- theorem rewrite_lift_k
+  --   [RenMap T [T]] [RenMapId T T] [RenMapCompose T T]
+  --   [SubstMap T [T]] [SubstMapId T T] [SubstMapCompose T T]
+  --   {k} {σ : Subst T}
+  --   : σ.lift k = 0..k ++ (σ ∘ +r k)
+  -- := by
+  --   induction k generalizing σ <;> simp
+  --   case _ k ih =>
+  --     rw [rewrite_lift_succ, ih]
+  --     simp; congr
 
-  @[simp, grind =]
-  theorem hrewrite1 [SubstMap S T] [SubstMapId S T] {σ : Subst S} : σ ◾ (id T) = σ := by
-    simp [hcompose, act, SubstAction.act]; congr
-    funext; case _ x =>
-    generalize zdef : σ.inner x = z
-    cases z <;> simp
+  -- @[simp, grind =]
+  -- theorem hrewrite1 [SubstMap S T] [SubstMapId S T] {σ : Subst S} : σ ◾ (id T) = σ := by
+  --   simp [hcompose, act, SubstAction.act]; congr
+  --   funext; case _ x =>
+  --   generalize zdef : σ.inner x = z
+  --   cases z <;> simp
 
-  @[simp, grind =]
-  theorem hrewrite1_ren [RenMap S T] [RenMapId S T] {σ : Subst S} : σ ◾ (.id T) = σ := by
-    simp [hcompose_ren, act, SubstAction.act]
+  -- @[simp, grind =]
+  -- theorem hrewrite1_ren [RenMap S T] [RenMapId S T] {σ : Subst S} : σ ◾ (.id T) = σ := by
+  --   simp [hcompose_ren, act, SubstAction.act]
 
-  @[simp, grind =]
-  theorem hrewrite2 [SubstMap S T] {σ : Subst T} : (id S) ◾ σ = +0σ := by
-    simp [hcompose, id, act, SubstAction.act]
+  -- @[simp, grind =]
+  -- theorem hrewrite2 [SubstMap S T] {σ : Subst T} : (id S) ◾ σ = +0σ := by
+  --   simp [hcompose, id, act, SubstAction.act]
 
-  @[simp, grind =]
-  theorem hrewrite2_ren [RenMap S T] {r : Ren T} : (id S) ◾ r = +0σ := by
-    simp [hcompose_ren, id, act, SubstAction.act]
+  -- @[simp, grind =]
+  -- theorem hrewrite2_ren [RenMap S T] {r : Ren T} : (id S) ◾ r = +0σ := by
+  --   simp [hcompose_ren, id, act, SubstAction.act]
 
-  @[simp, grind =]
-  theorem hrewrite3 [SubstMap S T] {σ : Subst T} : (succ S) ◾ σ = +1σ := by
-    simp [hcompose, succ, act, SubstAction.act]
+  -- @[simp, grind =]
+  -- theorem hrewrite3 [SubstMap S T] {σ : Subst T} : (succ S) ◾ σ = +1σ := by
+  --   simp [hcompose, succ, act, SubstAction.act]
 
-  @[simp, grind =]
-  theorem hrewrite3_ren [RenMap S T] {r : Ren T} : (succ S) ◾ r = +1σ := by
-    simp [hcompose_ren, succ, act, SubstAction.act]
+  -- @[simp, grind =]
+  -- theorem hrewrite3_ren [RenMap S T] {r : Ren T} : (succ S) ◾ r = +1σ := by
+  --   simp [hcompose_ren, succ, act, SubstAction.act]
 
-  @[simp, grind =]
-  theorem hrewrite4
-    [SubstMap S T]
-    {x} {σ : Subst S} {τ : Subst T}
-    : (re x :: σ) ◾ τ = re x :: (σ ◾ τ)
-  := by
-    simp [Subst.hcompose, act]; congr
-    funext; case _ i =>
-    cases i <;> simp [Subst.cons, act, SubstAction.act]
+  -- @[simp, grind =]
+  -- theorem hrewrite4
+  --   [SubstMap S T]
+  --   {x} {σ : Subst S} {τ : Subst T}
+  --   : (re x :: σ) ◾ τ = re x :: (σ ◾ τ)
+  -- := by
+  --   simp [Subst.hcompose, act]; congr
+  --   funext; case _ i =>
+  --   cases i <;> simp [Subst.cons, act, SubstAction.act]
 
-  @[simp, grind =]
-  theorem hrewrite4_ren
-    [RenMap S T]
-    {x} {σ : Subst S} {r : Ren T}
-    : (re x :: σ) ◾ r = re x :: (σ ◾ r)
-  := by
-    simp [hcompose_ren, act]; congr
-    funext; case _ i =>
-    cases i <;> simp [Subst.cons, act, SubstAction.act]
+  -- @[simp, grind =]
+  -- theorem hrewrite4_ren
+  --   [RenMap S T]
+  --   {x} {σ : Subst S} {r : Ren T}
+  --   : (re x :: σ) ◾ r = re x :: (σ ◾ r)
+  -- := by
+  --   simp [hcompose_ren, act]; congr
+  --   funext; case _ i =>
+  --   cases i <;> simp [Subst.cons, act, SubstAction.act]
 
-  @[grind =]
-  theorem hcomp_dist_ren_left
-    [SubstMap S T]
-    (r : Ren S) {σ : Subst S} {τ : Subst T}
-    : (r ∘ σ) ◾ τ = r ∘ σ ◾ τ
-  := by
-    funext; case _ x =>
-    simp [hcompose, compose_ren_left, act, SubstAction.act]
+  -- @[grind =]
+  -- theorem hcomp_dist_ren_left
+  --   [SubstMap S T]
+  --   (r : Ren S) {σ : Subst S} {τ : Subst T}
+  --   : (r ∘ σ) ◾ τ = r ∘ σ ◾ τ
+  -- := by
+  --   funext; case _ x =>
+  --   simp [hcompose, compose_ren_left, act, SubstAction.act]
 
-  @[simp, grind =]
-  theorem hrewrite5_subst_subst
-    [SubstMap S T] [SubstMap T T] [SubstMapCompose S T]
-    {σ : Subst S} {τ μ : Subst T}
-    : (σ ◾ τ) ◾ μ = σ ◾ (τ ∘ μ)
-  := by
-    simp [Subst.hcompose, act, SubstAction.act]
-    funext; case _ x =>
-    generalize zdef : σ.inner x = z
-    cases z <;> simp
+  -- @[simp, grind =]
+  -- theorem hrewrite5_subst_subst
+  --   [SubstMap S T] [SubstMap T [T]] [SubstMapCompose S T]
+  --   {σ : Subst S} {τ μ : Subst T}
+  --   : (σ ◾ τ) ◾ μ = σ ◾ (τ ∘ μ)
+  -- := by
+  --   simp [Subst.hcompose, act, SubstAction.act]
+  --   funext; case _ x =>
+  --   generalize zdef : σ.inner x = z
+  --   cases z <;> simp
 
-  @[simp, grind =]
-  theorem hrewrite5_subst_ren
-    [RenMap S T] [RenMap T T] [SubstMap S T] [SubstMapRenComposeRight S T]
-    {σ : Subst S} {τ : Subst T} {r : Ren T}
-    : (σ ◾ τ) ◾ r = σ ◾ (τ ∘ r)
-  := by
-    simp [hcompose_ren, hcompose, act, SubstAction.act]
-    funext; case _ x =>
-    generalize zdef : σ.inner x = z
-    cases z <;> simp
+  -- @[simp, grind =]
+  -- theorem hrewrite5_subst_ren
+  --   [RenMap S T] [RenMap T [T]] [SubstMap S T] [SubstMapRenComposeRight S T]
+  --   {σ : Subst S} {τ : Subst T} {r : Ren T}
+  --   : (σ ◾ τ) ◾ r = σ ◾ (τ ∘ r)
+  -- := by
+  --   simp [hcompose_ren, hcompose, act, SubstAction.act]
+  --   funext; case _ x =>
+  --   generalize zdef : σ.inner x = z
+  --   cases z <;> simp
 
-  @[simp, grind =]
-  theorem hrewrite5_ren_subst
-    [RenMap S T] [SubstMap S T] [SubstMapRenComposeLeft S T]
-    {σ : Subst S} {τ : Subst T} {r : Ren T}
-    : (σ ◾ r) ◾ τ = σ ◾ (r ∘ τ)
-  := by
-    simp [hcompose_ren, hcompose, act, SubstAction.act]
-    funext; case _ x =>
-    generalize zdef : σ.inner x = z
-    cases z <;> simp
+  -- @[simp, grind =]
+  -- theorem hrewrite5_ren_subst
+  --   [RenMap S T] [SubstMap S T] [SubstMapRenComposeLeft S T]
+  --   {σ : Subst S} {τ : Subst T} {r : Ren T}
+  --   : (σ ◾ r) ◾ τ = σ ◾ (r ∘ τ)
+  -- := by
+  --   simp [hcompose_ren, hcompose, act, SubstAction.act]
+  --   funext; case _ x =>
+  --   generalize zdef : σ.inner x = z
+  --   cases z <;> simp
 
-  @[simp, grind =]
-  theorem hrewrite5_ren_ren
-    [RenMap S T] [SubstMap S T] [RenMapCompose S T]
-    {σ : Subst S} {r1 r2 : Ren T}
-    : (σ ◾ r1) ◾ r2 = σ ◾ (r1 ∘ r2)
-  := by
-    simp [hcompose_ren, act, SubstAction.act]
+  -- @[simp, grind =]
+  -- theorem hrewrite5_ren_ren
+  --   [RenMap S T] [SubstMap S T] [RenMapCompose S T]
+  --   {σ : Subst S} {r1 r2 : Ren T}
+  --   : (σ ◾ r1) ◾ r2 = σ ◾ (r1 ∘ r2)
+  -- := by
+  --   simp [hcompose_ren, act, SubstAction.act]
 
-  @[grind =]
-  theorem hcomp_distr_ren_right
-    [RenMap S S] [RenMap S T] [SubstMap S S] [SubstMap S T] [SubstMapRenCommute S T]
-    (r : Ren S) (σ : Subst S) (μ : Subst T)
-    : (σ ∘ r) ◾ μ = (σ ◾ μ) ∘ r
-  := by
-    simp [hcompose, compose_ren_right, act, SubstAction.act]; funext; case _ x =>
-    generalize zdef : σ.inner x = z
-    cases z <;> simp
-    rw [apply_commute_ren_subst]
+  -- @[grind =]
+  -- theorem hcomp_distr_ren_right
+  --   [RenMap S S] [RenMap S T] [SubstMap S S] [SubstMap S T] [SubstMapRenCommute S T]
+  --   (r : Ren S) (σ : Subst S) (μ : Subst T)
+  --   : (σ ∘ r) ◾ μ = (σ ◾ μ) ∘ r
+  -- := by
+  --   simp [hcompose, compose_ren_right, act, SubstAction.act]; funext; case _ x =>
+  --   generalize zdef : σ.inner x = z
+  --   cases z <;> simp
+  --   rw [apply_commute_ren_subst]
 
-  @[simp, grind =]
-  theorem hrewrite7
-    [SubstMap S S] [SubstMap S T] [SubstMapHetCompose S T]
-    {σ τ : Subst S} (μ : Subst T)
-    : (σ ∘ τ) ◾ μ = (σ ◾ μ) ∘ τ ◾ μ
-  := by
-    simp [hcompose, compose, act, SubstAction.act]
-    funext; case _ x =>
-    generalize zdef : σ.inner x = z
-    cases z <;> simp [hcompose, act, SubstAction.act]
+  -- @[simp, grind =]
+  -- theorem hrewrite7
+  --   [SubstMap S S] [SubstMap S T] [SubstMapHetCompose S T]
+  --   {σ τ : Subst S} (μ : Subst T)
+  --   : (σ ∘ τ) ◾ μ = (σ ◾ μ) ∘ τ ◾ μ
+  -- := by
+  --   simp [hcompose, compose, act, SubstAction.act]
+  --   funext; case _ x =>
+  --   generalize zdef : σ.inner x = z
+  --   cases z <;> simp [hcompose, act, SubstAction.act]
 
-  @[simp, grind =]
-  theorem hrewrite7_ren
-    [RenMap S S] [RenMap S T] [SubstMap S S] [SubstMap S T] [SubstMapRenHetCompose S T]
-    {σ τ : Subst S} {r : Ren T}
-    : (σ ∘ τ) ◾ r = (σ ◾ r) ∘ τ ◾ r
-  := by
-    simp [hcompose_ren, compose, act, SubstAction.act]
-    funext; case _ x =>
-    generalize zdef : σ.inner x = z
-    cases z <;> simp [hcompose_ren, act, SubstAction.act]
+  -- @[simp, grind =]
+  -- theorem hrewrite7_ren
+  --   [RenMap S S] [RenMap S T] [SubstMap S S] [SubstMap S T] [SubstMapRenHetCompose S T]
+  --   {σ τ : Subst S} {r : Ren T}
+  --   : (σ ∘ τ) ◾ r = (σ ◾ r) ∘ τ ◾ r
+  -- := by
+  --   simp [hcompose_ren, compose, act, SubstAction.act]
+  --   funext; case _ x =>
+  --   generalize zdef : σ.inner x = z
+  --   cases z <;> simp [hcompose_ren, act, SubstAction.act]
 
-  @[simp, grind =]
-  theorem hrewrite8
-    [SubstMap S S] [SubstMap S T]
-    {r : Ren S} {τ : Subst S} (μ : Subst T)
-    : (r ∘ τ) ◾ μ = r ∘ τ ◾ μ
-  := by
-    simp [hcompose, compose_ren_left, act, SubstAction.act]
+  -- @[simp, grind =]
+  -- theorem hrewrite8
+  --   [SubstMap S S] [SubstMap S T]
+  --   {r : Ren S} {τ : Subst S} (μ : Subst T)
+  --   : (r ∘ τ) ◾ μ = r ∘ τ ◾ μ
+  -- := by
+  --   simp [hcompose, compose_ren_left, act, SubstAction.act]
 
-  @[simp, grind =]
-  theorem hrewrite8_ren
-    [RenMap S T] [SubstMap S S] [SubstMap S T]
-    {r : Ren S} {τ : Subst S} (μ : Ren T)
-    : (r ∘ τ) ◾ μ = r ∘ τ ◾ μ
-  := by
-    simp [hcompose_ren, compose_ren_left, act, SubstAction.act]
+  -- @[simp, grind =]
+  -- theorem hrewrite8_ren
+  --   [RenMap S T] [SubstMap S S] [SubstMap S T]
+  --   {r : Ren S} {τ : Subst S} (μ : Ren T)
+  --   : (r ∘ τ) ◾ μ = r ∘ τ ◾ μ
+  -- := by
+  --   simp [hcompose_ren, compose_ren_left, act, SubstAction.act]
 
-  @[simp, grind =]
-  theorem hrewrite9
-    [RenMap S S] [RenMap S T] [SubstMap S S] [SubstMap S T] [SubstMapRenCommute S T]
-    {σ : Subst S} {r : Ren S} (μ : Subst T)
-    : (σ ∘ r) ◾ μ = (σ ◾ μ) ∘ r
-  := by
-    simp [hcompose, compose_ren_right, act, SubstAction.act]
-    funext; case _ x =>
-    generalize zdef : σ.inner x = z
-    cases z <;> simp
-    rw [apply_commute_ren_subst]
+  -- @[simp, grind =]
+  -- theorem hrewrite9
+  --   [RenMap S S] [RenMap S T] [SubstMap S S] [SubstMap S T] [SubstMapRenCommute S T]
+  --   {σ : Subst S} {r : Ren S} (μ : Subst T)
+  --   : (σ ∘ r) ◾ μ = (σ ◾ μ) ∘ r
+  -- := by
+  --   simp [hcompose, compose_ren_right, act, SubstAction.act]
+  --   funext; case _ x =>
+  --   generalize zdef : σ.inner x = z
+  --   cases z <;> simp
+  --   rw [apply_commute_ren_subst]
 
-  @[simp, grind =]
-  theorem hrewrite9_ren
-    [RenMap S S] [RenMap S T] [SubstMap S S] [SubstMap S T] [SubstMapRenCommute S T]
-    {σ : Subst S} {r : Ren S} (μ : Ren T)
-    : (σ ∘ r) ◾ μ = (σ ◾ μ) ∘ r
-  := by
-    simp [hcompose_ren, compose_ren_right, act, SubstAction.act]
-    funext; case _ x =>
-    generalize zdef : σ.inner x = z
-    cases z <;> simp
-    rw [apply_commute_ren_ren]
+  -- @[simp, grind =]
+  -- theorem hrewrite9_ren
+  --   [RenMap S S] [RenMap S T] [SubstMap S S] [SubstMap S T] [SubstMapRenCommute S T]
+  --   {σ : Subst S} {r : Ren S} (μ : Ren T)
+  --   : (σ ∘ r) ◾ μ = (σ ◾ μ) ∘ r
+  -- := by
+  --   simp [hcompose_ren, compose_ren_right, act, SubstAction.act]
+  --   funext; case _ x =>
+  --   generalize zdef : σ.inner x = z
+  --   cases z <;> simp
+  --   rw [apply_commute_ren_ren]
 
-  theorem hrewrite_lift1
-    [RenMap S S] [RenMap S T] [SubstMap S S] [SubstMap S T] [SubstMapRenCommute S T]
-    {σ : Subst S} {τ : Subst T}
-    : (σ ◾ τ).lift = σ.lift ◾ τ
-  := by
-    simp [lift, act, SubstAction.act]; congr; funext; case _ i =>
-    cases i <;> simp [act, SubstAction.act]
-    case _ n =>
-      simp [hcompose, act, SubstAction.act]
-      generalize zdef : σ.inner n = z
-      cases z <;> simp; case _ t =>
-      rw [apply_commute_ren_subst]
+  -- theorem hrewrite_lift1
+  --   [RenMap S S] [RenMap S T] [SubstMap S S] [SubstMap S T] [SubstMapRenCommute S T]
+  --   {σ : Subst S} {τ : Subst T}
+  --   : (σ ◾ τ).lift = σ.lift ◾ τ
+  -- := by
+  --   simp [lift, act, SubstAction.act]; congr; funext; case _ i =>
+  --   cases i <;> simp [act, SubstAction.act]
+  --   case _ n =>
+  --     simp [hcompose, act, SubstAction.act]
+  --     generalize zdef : σ.inner n = z
+  --     cases z <;> simp; case _ t =>
+  --     rw [apply_commute_ren_subst]
 
-  @[simp, grind =]
-  theorem hrewrite_lift
-    [RenMap S S] [RenMap S T] [SubstMap S S] [SubstMap S T]
-    [RenMapId S S] [RenMapCompose S S] [SubstMapRenCommute S T]
-    {k} {σ : Subst S} {τ : Subst T}
-    : (σ ◾ τ).lift k = σ.lift k ◾ τ
-  := by
-    induction k generalizing σ τ
-    case _ => simp
-    case _ i ih =>
-      rw [rewrite_lift_succ]
-      rw [rewrite_lift_succ]
-      simp; rw [ih]
-      grind
+  -- @[simp, grind =]
+  -- theorem hrewrite_lift
+  --   [RenMap S S] [RenMap S T] [SubstMap S S] [SubstMap S T]
+--     [RenMapId S S] [RenMapCompose S S] [SubstMapRenCommute S T]
+--     {k} {σ : Subst S} {τ : Subst T}
+--     : (σ ◾ τ).lift k = σ.lift k ◾ τ
+--   := by
+--     induction k generalizing σ τ
+--     case _ => simp
+--     case _ i ih =>
+--       rw [rewrite_lift_succ]
+--       rw [rewrite_lift_succ]
+--       simp; rw [ih]
+--       grind
 
-  theorem hrewrite_lift1_ren
-    [RenMap S S] [SubstMap S S] [RenMap S T] [SubstMap S T] [SubstMapRenCommute S T]
-    {σ : Subst S} {τ : Ren T}
-    : (σ ◾ τ).lift = σ.lift ◾ τ
-  := by
-    simp [lift, act, SubstAction.act]; congr; funext; case _ i =>
-    cases i <;> simp [act, SubstAction.act]
-    case _ n =>
-      simp [hcompose_ren, act, SubstAction.act]
-      generalize zdef : σ.inner n = z
-      cases z <;> simp; case _ t =>
-      rw [apply_commute_ren_ren]
+--   theorem hrewrite_lift1_ren
+--     [RenMap S S] [SubstMap S S] [RenMap S T] [SubstMap S T] [SubstMapRenCommute S T]
+--     {σ : Subst S} {τ : Ren T}
+--     : (σ ◾ τ).lift = σ.lift ◾ τ
+--   := by
+--     simp [lift, act, SubstAction.act]; congr; funext; case _ i =>
+--     cases i <;> simp [act, SubstAction.act]
+--     case _ n =>
+--       simp [hcompose_ren, act, SubstAction.act]
+--       generalize zdef : σ.inner n = z
+--       cases z <;> simp; case _ t =>
+--       rw [apply_commute_ren_ren]
 
-  @[simp, grind =]
-  theorem hrewrite_lift_ren
-    [RenMap S S] [RenMap S T] [SubstMap S S] [SubstMap S T]
-    [RenMapId S S] [RenMapCompose S S] [SubstMapRenCommute S T]
-    {k} {σ : Subst S} {τ : Ren T}
-    : (σ ◾ τ).lift k = σ.lift k ◾ τ
-  := by
-    induction k generalizing σ τ
-    case _ => simp
-    case _ i ih =>
-      rw [rewrite_lift_succ]
-      rw [rewrite_lift_succ (k := i)]
-      simp; rw [ih]
-end Subst
+--   @[simp, grind =]
+--   theorem hrewrite_lift_ren
+--     [RenMap S S] [RenMap S T] [SubstMap S S] [SubstMap S T]
+--     [RenMapId S S] [RenMapCompose S S] [SubstMapRenCommute S T]
+--     {k} {σ : Subst S} {τ : Ren T}
+--     : (σ ◾ τ).lift k = σ.lift k ◾ τ
+--   := by
+--     induction k generalizing σ τ
+--     case _ => simp
+--     case _ i ih =>
+--       rw [rewrite_lift_succ]
+--       rw [rewrite_lift_succ (k := i)]
+--       simp; rw [ih]
+-- end Subst
 
-@[grind =]
-theorem Subst.compose_commute_succ [RenMap T T] {τ : Subst T}
-  : τ ∘ Ren.succ T = Ren.succ T ∘ τ.lift
-:= by congr
+-- @[grind =]
+-- theorem Subst.compose_commute_succ [RenMap T [T]] {τ : Subst T}
+--   : τ ∘ Ren.succ T = Ren.succ T ∘ τ.lift
+-- := by congr
 
-@[grind =]
-theorem Ren.compose_commute_succ {r : Ren T} : r ∘ succ T = succ T ∘ r.lift := by simp [compose]
+-- @[grind =]
+-- theorem Ren.compose_commute_succ {r : Ren T} : r ∘ succ T = succ T ∘ r.lift := by simp [compose]
 
-theorem Subst.rewrite_lift_compose_ren_left_k1 [RenMap T T] {r : Ren T} {τ : Subst T}
-  : (r ∘ τ).lift = r.lift ∘ τ.lift
-:= by
-  simp [compose_ren_left, lift, Ren.lift, act, SubstAction.act]
-  funext; case _ x =>
-  cases x <;> simp
+-- theorem Subst.rewrite_lift_compose_ren_left_k1 [RenMap T [T]] {r : Ren T} {τ : Subst T}
+--   : (r ∘ τ).lift = r.lift ∘ τ.lift
+-- := by
+--   simp [compose_ren_left, lift, Ren.lift, act, SubstAction.act]
+--   funext; case _ x =>
+--   cases x <;> simp
 
-@[simp, grind =]
-theorem Subst.rewrite_lift_compose_ren_left
-  [RenMap T T] [RenMapId T T] [RenMapCompose T T]
-  {k} {r : Ren T} {τ : Subst T}
-  : (r ∘ τ).lift k = r.lift k ∘ τ.lift k
-:= by
-  induction k generalizing r τ; congr
-  case _ k ih =>
-    rw [rewrite_lift_succ, ih]
-    rw [rewrite_lift_compose_ren_left_k1]
-    rw [<-rewrite_lift_succ]
-    rw [<-Ren.lift_of_succ]
+-- @[simp, grind =]
+-- theorem Subst.rewrite_lift_compose_ren_left
+--   [RenMap T [T]] [RenMapId T T] [RenMapCompose T T]
+--   {k} {r : Ren T} {τ : Subst T}
+--   : (r ∘ τ).lift k = r.lift k ∘ τ.lift k
+-- := by
+--   induction k generalizing r τ; congr
+--   case _ k ih =>
+--     rw [rewrite_lift_succ, ih]
+--     rw [rewrite_lift_compose_ren_left_k1]
+--     rw [<-rewrite_lift_succ]
+--     rw [<-Ren.lift_of_succ]
 
-theorem Subst.lift_compose_ren_right_k1
-  [RenMap T T] [RenMapId T T] [RenMapCompose T T]
-  {σ : Subst T} {r : Ren T}
-  : (σ ∘ r).lift = σ.lift ∘ r.lift
-:= by
-  simp [lift, act, SubstAction.act]; congr; funext; case _ x =>
-  cases x <;> simp [act, SubstAction.act]; case _ x =>
-  simp [compose_ren_right, act, SubstAction.act]; grind
+-- theorem Subst.lift_compose_ren_right_k1
+--   [RenMap T [T]] [RenMapId T T] [RenMapCompose T T]
+--   {σ : Subst T} {r : Ren T}
+--   : (σ ∘ r).lift = σ.lift ∘ r.lift
+-- := by
+--   simp [lift, act, SubstAction.act]; congr; funext; case _ x =>
+--   cases x <;> simp [act, SubstAction.act]; case _ x =>
+--   simp [compose_ren_right, act, SubstAction.act]; grind
 
-@[simp, grind =]
-theorem Subst.lift_compose_ren_right
-  [RenMap T T] [RenMapId T T] [RenMapCompose T T]
-  {k} {σ : Subst T} {r : Ren T}
-  : (σ ∘ r).lift k = σ.lift k ∘ r.lift k
-:= by
-  induction k generalizing σ r; simp
-  case _ k ih =>
-    rw [rewrite_lift_succ, ih]
-    rw [lift_compose_ren_right_k1]
-    rw [<-rewrite_lift_succ]
-    rw [<-Ren.lift_of_succ]
+-- @[simp, grind =]
+-- theorem Subst.lift_compose_ren_right
+--   [RenMap T [T]] [RenMapId T T] [RenMapCompose T T]
+--   {k} {σ : Subst T} {r : Ren T}
+--   : (σ ∘ r).lift k = σ.lift k ∘ r.lift k
+-- := by
+--   induction k generalizing σ r; simp
+--   case _ k ih =>
+--     rw [rewrite_lift_succ, ih]
+--     rw [lift_compose_ren_right_k1]
+--     rw [<-rewrite_lift_succ]
+--     rw [<-Ren.lift_of_succ]
 
-theorem Subst.rewrite_lift_compose_k1
-  [RenMap T T] [SubstMap T T] [SubstMapRenComposeLeft T T] [SubstMapRenComposeRight T T]
-  {σ τ : Subst T}
-  : (σ ∘ τ).lift = σ.lift ∘ τ.lift
-:= by
-  simp [compose, lift, act, SubstAction.act]
-  funext; case _ x =>
-  cases x <;> simp [act, SubstAction.act]
-  case _ x =>
-  cases σ.inner x <;> simp [act, SubstAction.act]; case _ t =>
-  have lem := Subst.compose_commute_succ (τ := τ)
-  simp [lift, act, SubstAction.act] at lem
-  rw [lem]
+-- theorem Subst.rewrite_lift_compose_k1
+--   [RenMap T [T]] [SubstMap T [T]] [SubstMapRenComposeLeft T T] [SubstMapRenComposeRight T T]
+--   {σ τ : Subst T}
+--   : (σ ∘ τ).lift = σ.lift ∘ τ.lift
+-- := by
+--   simp [compose, lift, act, SubstAction.act]
+--   funext; case _ x =>
+--   cases x <;> simp [act, SubstAction.act]
+--   case _ x =>
+--   cases σ.inner x <;> simp [act, SubstAction.act]; case _ t =>
+--   have lem := Subst.compose_commute_succ (τ := τ)
+--   simp [lift, act, SubstAction.act] at lem
+--   rw [lem]
 
-@[simp, grind =]
-theorem Subst.rewrite_lift_compose
-  [RenMap T T] [RenMapId T T] [RenMapCompose T T] [SubstMap T T]
-  [SubstMapRenComposeLeft T T] [SubstMapRenComposeRight T T]
-  {k} {σ τ : Subst T}
-  : (σ ∘ τ).lift k = σ.lift k ∘ τ.lift k
-:= by
-  induction k generalizing σ τ; simp
-  case _ k ih =>
-    rw [rewrite_lift_succ, ih]
-    rw [rewrite_lift_succ (σ := σ)]
-    rw [rewrite_lift_succ (σ := τ)]
-    rw [rewrite_lift_compose_k1]
+-- @[simp, grind =]
+-- theorem Subst.rewrite_lift_compose
+--   [RenMap T [T]] [RenMapId T T] [RenMapCompose T T] [SubstMap T [T]]
+--   [SubstMapRenComposeLeft T T] [SubstMapRenComposeRight T T]
+--   {k} {σ τ : Subst T}
+--   : (σ ∘ τ).lift k = σ.lift k ∘ τ.lift k
+-- := by
+--   induction k generalizing σ τ; simp
+--   case _ k ih =>
+--     rw [rewrite_lift_succ, ih]
+--     rw [rewrite_lift_succ (σ := σ)]
+--     rw [rewrite_lift_succ (σ := τ)]
+--     rw [rewrite_lift_compose_k1]
 
 end LeanSubst
