LeanSubst/Types/Nat.lean
@@ -6,13 +6,13 @@ namespace LeanSubst
 universe u1 u2 u3
 variable {S : Type u1} {T : Type u2} {U : Type u3}
 
-def Nat.rmap (r : Ren T) : Nat -> Nat
-| n => r.act n
+-- def Nat.rmap (r : Ren T) : Nat -> Nat
+-- | n => r.act n
 
-instance : RenMap Nat T where
-  rmap := Nat.rmap
+-- instance : RenMap Nat T where
+--   rmap := Nat.rmap
 
-@[simp, grind =]
-theorem Nat.rmap_simp {r : Ren T} {n} : n⟨r⟩ = r.act n := by simp [RenMap.rmap, Nat.rmap]
+-- @[simp, grind =]
+-- theorem Nat.rmap_simp {r : Ren T} {n} : n⟨r⟩ = r.act n := by simp [RenMap.rmap, Nat.rmap]
 
 end LeanSubst
